LogRelFI/ValidPTy.v
@@ -1,0 +1,119 @@
+Require Export LogRelFI.PseudoType.
+Require Export RecTypes.Contraction.
+Require Export LogRelFI.Contraction.
+
+Require Import Coq.Bool.Bool.
+Require Import Coq.Arith.Max.
+Require Import Coq.micromega.Lia.
+
+Fixpoint pNumbFree (τ : PTy) : nat :=
+  match τ with
+  | ptunit => 0
+  | ptbool => 0
+  | ptprod τ1 τ2 => max (pNumbFree τ1) (pNumbFree τ2)
+  | ptsum τ1 τ2 => max (pNumbFree τ1) (pNumbFree τ2)
+  | ptarr τ1 τ2 => max (pNumbFree τ1) (pNumbFree τ2)
+  | pEmulDV n p τ => 0
+  end.
+Arguments pNumbFree !τ.
+
+Lemma pNumbFree_sound τ : innerPClosed τ → ws (pNumbFree τ) τ.
+Proof.
+  induction τ; cbn; try constructor; dependent destruction H.
+  - refine (WsPTy_mono _ (IHτ1 H)); lia.
+  - refine (WsPTy_mono _ (IHτ2 H)); lia.
+  - refine (WsPTy_mono _ (IHτ1 H)); lia.
+  - refine (WsPTy_mono _ (IHτ2 H)); lia.
+  - refine (WsPTy_mono _ (IHτ1 H)); lia.
+  - refine (WsPTy_mono _ (IHτ2 H)); lia.
+  - assumption.
+Qed.
+
+Definition pDecideClosed τ := match pNumbFree τ with
+                             | 0 => B.true
+                             | _ => B.false
+                             end.
+
+Arguments pDecideClosed /.
+Lemma decidePClosed_sound {τ} : innerPClosed τ → Is_true (pDecideClosed τ) -> ⟨ 0 ⊢ τ ⟩.
+Proof.
+  unfold pDecideClosed, WsTy.
+  remember (pNumbFree τ).
+  destruct n; intuition.
+  rewrite Heqn.
+  now eapply pNumbFree_sound.
+Qed.
+
+Lemma pNumbFree_complete {τ n} : ⟨ n ⊢ τ ⟩ -> pNumbFree τ <= n.
+Proof.
+  induction 1; cbn; try lia.
+Qed.
+
+Lemma pNumbFree_complete' {τ} : ⟨ 0 ⊢ τ ⟩ -> pNumbFree τ = 0.
+Proof.
+  intros cl.
+  cut (pNumbFree τ <= 0).
+  - lia.
+  - now eapply pNumbFree_complete.
+Qed.
+
+Lemma pDecideClosed_complete {τ} : ⟨ 0 ⊢ τ ⟩ -> Is_true (pDecideClosed τ).
+Proof.
+  intros cτ.
+  assert (nc := pNumbFree_complete cτ).
+  assert (eq : pNumbFree τ = 0) by lia.
+  unfold pDecideClosed.
+  now rewrite eq.
+Qed.
+
+Inductive ClosedPEnv : PEnv → Prop :=
+  | PEmptyClosed : ClosedPEnv pempty
+  | VarPClosed {Γ τ} :
+      ⟨ 0 ⊢ τ ⟩ →
+      ClosedPEnv Γ →
+      ClosedPEnv (Γ p▻ τ).
+
+Hint Constructors wsPTy : cty.
+Hint Constructors ClosedPEnv : cenv.
+
+Definition ValidPTy : PTy -> Prop := fun τ => ⟨ 0 ⊢ τ ⟩ /\ SimplePContr τ.
+(* Definition ValidPEnv : PEnv -> Prop := fun Γ => ClosedPEnv Γ /\ ContrPEnv Γ. *)
+
+Lemma ValidPTy_SimplePContr {τ} : ValidPTy τ -> SimplePContr τ.
+Proof.
+  now destruct 1.
+Qed.
+Hint Resolve ValidPTy_SimplePContr : simple_p_contr_rec.
+
+(* Lemma ValidPEnv_nil : ValidPEnv pempty. *)
+(* Proof. *)
+(*   split; constructor; eauto. *)
+(* Qed. *)
+(* Hint Resolve ValidPEnv_nil : ptyvalid. *)
+
+(* Lemma ValidPEnv_cons {Γ τ} : ValidPEnv Γ -> ValidPTy τ -> ValidPEnv (Γ p▻ τ). *)
+(* Proof. *)
+(*   intros [env_cl env_contr] [ty_cl ty_contr]. *)
+(*   split; constructor; eauto. *)
+(* Qed. *)
+(* Hint Resolve ValidPEnv_cons : ptyvalid. *)
+
+(* Lemma ValidPEnv_invert_cons {Γ τ} : ValidPEnv (Γ p▻ τ) → ValidPEnv Γ ∧ ValidPTy τ. *)
+(* Proof. *)
+(*   intro vΓ. *)
+(*   destruct vΓ as (closedΓ & contrΓ). *)
+(*   inversion closedΓ; inversion contrΓ; subst. *)
+(*   split; split; assumption. *)
+(* Qed. *)
+
+(* Lemma ValidPEnv_getevar {Γ i τ} : ValidPEnv Γ → ⟪ i : τ p∈ Γ ⟫ → ValidPTy τ. *)
+(* Proof. *)
+(*   revert Γ. *)
+(*   induction i; intros Γ vΓ ev. *)
+(*   - inversion ev; subst. *)
+(*     destruct (ValidPEnv_invert_cons vΓ) as (_ & vτ). *)
+(*     assumption. *)
+(*   - inversion ev; subst. *)
+(*     destruct (ValidPEnv_invert_cons vΓ) as (vΓ0 & _). *)
+(*     apply (IHi Γ0 vΓ0 H1). *)
+(* Qed. *)
